txn-data-consistency/EP+_Refinement_Proof.thy
@@ -1979,283 +1979,6 @@ lemma t_is_fresh:
   by (auto simp add: kvs_of_s_defs next_txids_def)
 
 
-subsection \<open>Closedness\<close>
-
-lemma visTx'_union_distr: "visTx' K (u\<^sub>1 \<union> u\<^sub>2) = visTx' K u\<^sub>1 \<union> visTx' K u\<^sub>2"
-  by (auto simp add: visTx'_def)
-
-lemma visTx'_Union_distr: "visTx' K (\<Union>i\<in>I. u i) = (\<Union>i\<in>I. visTx' K (u i))"
-  by (auto simp add: visTx'_def)
-
-lemma visTx'_same_writers: "kvs_writers K' = kvs_writers K \<Longrightarrow> visTx' K' u = visTx' K u"
-  by (simp add: visTx'_def)
-
-lemma union_closed':
-  assumes "closed' K u\<^sub>1 r"
-    and "closed' K u\<^sub>2 r"
-    and "kvs_writers K' = kvs_writers K" 
-    and "read_only_Txs K \<subseteq> read_only_Txs K'"
-  shows "closed' K' (u\<^sub>1 \<union> u\<^sub>2) r"
-  using assms
-  by (auto simp add: closed'_def visTx'_union_distr visTx'_same_writers[of K']
-           intro: closed_general_set_union_closed)
-
-lemma Union_closed':
-  assumes "\<And>i. i \<in> I \<Longrightarrow> closed' K (u i) r"
-    and "finite I" 
-    and "kvs_writers K' = kvs_writers K" 
-    and "read_only_Txs K \<subseteq> read_only_Txs K'"
-  shows "closed' K' (\<Union>i\<in>I. u i) r"
-  using assms                                  
-  apply (simp add: closed'_def visTx'_Union_distr visTx'_same_writers[of K'])
-  apply (rule closed_general_set_Union_closed)
-  apply auto
-  done
-
-lemma union_closed'_extend_rel:
-  assumes "closed' K u\<^sub>1 r"
-    and "closed' K u\<^sub>2 r"
-    and "kvs_writers K' = kvs_writers K" 
-    and "read_only_Txs K \<subseteq> read_only_Txs K'"
-    and "x \<notin> (r\<inverse>)\<^sup>* `` (visTx' K u\<^sub>1 \<union> visTx' K u\<^sub>2)"
-    and "r' = (\<Union>y\<in>Y. {(y, x)}) \<union> r"
-    and "finite Y"
-  shows "closed' K' (u\<^sub>1 \<union> u\<^sub>2) r'"
-  using assms
-  by (auto simp add: closed'_def visTx'_union_distr visTx'_same_writers[of K']
-      intro: closed_general_union_V_extend_N_extend_rel)
-
-
-lemma visTx'_new_writer: "kvs_writers K' = insert t (kvs_writers K) \<Longrightarrow>
-  visTx' K' (insert t u) = insert t (visTx' K u)"
-  by (auto simp add: visTx'_def)
-
-lemma insert_wr_t_closed':
-  assumes "closed' K u r"
-    and "closed_general {t} (r\<inverse>) (visTx' K u \<union> read_only_Txs K)"
-    and "read_only_Txs K' = read_only_Txs K"
-    and "kvs_writers K' = insert t (kvs_writers K)"
-  shows "closed' K' (insert t u) r"
-  using assms
-  by (auto simp add: closed'_def visTx'_new_writer intro: closed_general_set_union_closed)
-
-\<comment> \<open>insert (k, t) in version's deps - used in get_ctx\<close>
-lemma visTx'_observes_t:
-  "t \<in> kvs_writers K \<Longrightarrow> visTx' K (insert t u) = insert t (visTx' K u)"
-  by (simp add: visTx'_def)
-
-lemma insert_kt_to_u_closed':
-  assumes "closed' K u r"
-    and "t \<in> kvs_writers K"
-    and "closed_general {t} (r\<inverse>) (visTx' K u \<union> read_only_Txs K)"
-  shows "closed' K (insert t u) r"
-  using assms
-  by (auto simp add: closed'_def visTx'_observes_t intro: closed_general_set_union_closed)
-
-
-\<comment> \<open>concrete cl_read_done closedness\<close>
-
-\<comment> \<open>premises\<close>
- 
-lemma v_writer_kvs_of_s:
-  assumes "reach tps_s s"
-  shows "v_writer ` set (kvs_of_s s k) = set (cts_order s k)"
-  using assms CO_not_No_Ver_def[of s]
-  by (auto simp add: kvs_of_s_defs image_iff split: ver_state.split)
-
-lemma v_readerset_kvs_of_s:
-  assumes "reach tps_s s"
-  shows "\<Union> (v_readerset ` set (kvs_of_s s k)) = 
-   {t. \<exists>t_wr \<in> set (cts_order s k).
-      \<exists>cts sts lst v rs rts rlst. svr_state (svrs s k) t_wr = Commit cts sts lst v rs \<and>
-      rs t = Some (rts, rlst) \<and> get_sn t < cl_sn (cls s (get_cl t))}"
-  using assms CO_not_No_Ver_def[of s]
-  apply (auto simp add: kvs_of_s_defs split: ver_state.split ver_state.split_asm)
-  by blast
-
-lemma v_writer_kvs_of_s_nth:
-  "reach tps_s s \<Longrightarrow> i < length (kvs_of_s s k) \<Longrightarrow> v_writer (kvs_of_s s k ! i) = cts_order s k ! i"
-  using CO_not_No_Ver_def[of s k]
-  by (auto simp add: kvs_of_s_defs split: ver_state.split)
-
-lemma v_readerset_kvs_of_s_nth:
-  "reach tps_s s \<Longrightarrow> i < length (cts_order s k) \<Longrightarrow>
-    v_readerset (kvs_of_s s k ! i) = get_abst_rs s k (cts_order s k ! i)"
-  using CO_not_No_Ver_def[of s k]
-  by (auto simp add: kvs_of_s_defs split: ver_state.split)
-
-lemma cl_read_done_same_writers:
-  assumes "reach tps_s s"
-    and "cl_read_done_s cl kv_map sn u'' clk s s'"
-  shows "kvs_writers (kvs_of_s s') = kvs_writers (kvs_of_s s)"
-proof -
-  have "reach tps_s s'"
-    using assms reach.reach_trans[of tps_s s "RDone cl kv_map sn u'' clk" s'] by auto
-  then show ?thesis
-    using assms CO_not_No_Ver_def[of s]
-    apply (simp add: kvs_writers_def vl_writers_def v_writer_kvs_of_s)
-    by (simp add: cl_read_done_s_def cl_read_done_U_def)
-qed
-
-lemma insert_Diff_if': "a \<notin> c \<Longrightarrow> insert a (b - c) = insert a b - c"
-  by (simp add: insert_Diff_if)
-
-lemma cl_read_done_t_notin_kvs_writers:
-  assumes "reach tps_s s"
-    and "cl_read_done_s cl kv_map sn u'' clk s s'"
-  shows "Tn (get_txn s cl) \<notin> kvs_writers (kvs_of_s s)"
-  using assms
-  apply (simp add: kvs_writers_def vl_writers_def v_writer_kvs_of_s)
-  using CO_Tid_def[of s cl] 
-  apply (auto simp add: tps_trans_defs)
-  by blast
-
-lemma UNIV_ex: "(\<Union>x. {t. P t x}) = ({t. \<exists>x. P t x})"
-  by auto
-
-lemma cl_read_done_new_read:
-  assumes "reach tps_s s"
-    and "cl_read_done_s cl kv_map sn u'' clk s s'"
-  shows "read_only_Txs (kvs_of_s s') = insert (Tn (get_txn s cl)) (read_only_Txs (kvs_of_s s))"
-proof -
-  have reach_s': "reach tps_s s'" 
-    using assms reach.reach_trans[of tps_s s "RDone cl kv_map sn u'' clk" s'] by auto
-  show ?thesis
-  using assms cl_read_done_t_notin_kvs_writers[OF assms] cl_read_done_same_writers[OF assms(1)]
-  apply (simp add: read_only_Txs_def insert_Diff_if')
-  apply (rule arg_cong[where f="\<lambda>m. m - _"])
-  apply (simp add: kvs_readers_def vl_readers_def v_readerset_kvs_of_s[OF assms(1)]
-      v_readerset_kvs_of_s[OF reach_s'] UNIV_ex)
-  using CO_not_No_Ver_def[of s']
-  apply (auto simp add: tps_trans_defs image_insert[symmetric] simp del: image_insert)
-  using image_eqI apply blast
-  apply (smt (z3) image_eqI insertCI less_SucE mem_Collect_eq txid0.collapse)
-  using image_eqI apply blast
-  subgoal apply (rule image_eqI, auto)
-    using Finite_Dom_Kv_map_rd_def[of s cl]
-    apply (cases "dom kv_map = {}", auto simp add: ex_in_conv[symmetric] simp del: dom_eq_empty_conv)
-    subgoal for k v apply (rule exI[where x=k])
-      using Rtxn_RegK_Kvtm_Cmt_in_rs_def[of s cl] Committed_Abs_in_CO_def[of s]
-      apply (auto simp add: is_committed_in_kvs_def)
-      by (metis (no_types, lifting) is_committed.simps(1))
-    done
-  by (smt (verit) image_eqI less_Suc_eq mem_Collect_eq)
-qed
-
-lemma fresh_rtxn_not_vis:
-  assumes "Tn (get_txn s cl) \<notin> kvs_writers (kvs_of_s s)"
-    and "\<forall>t \<in> kvs_writers (kvs_of_s s). get_sn_w t < cl_sn (cls s cl)"
-  shows "Tn (get_txn s cl) \<notin> ((R_CC (kvs_of_s s))\<inverse>)\<^sup>* `` (visTx' (kvs_of_s s)
-    (\<Union>k. get_view s cl k))"
-  apply (auto simp add: visTx'_def R_CC_def)
-  subgoal for t apply (induction t "Tn (get_txn s cl)" rule: rtrancl.induct, auto)
-      apply (simp add: assms(1))
-     apply (simp add: SO_def SO0_def) oops
-
-definition wtxns_readable :: "('v, 'm) global_conf_scheme \<Rightarrow> cl_id \<Rightarrow> key set \<Rightarrow> txid set" where
-  "wtxns_readable s cl keys \<equiv> {read_at (svr_state (svrs s k)) (gst (cls s cl)) cl | k. k \<in> keys}"
-
-lemma finite_wtxns_readable: "finite keys \<longrightarrow> finite (wtxns_readable s cl keys)"
-  by (simp add: wtxns_readable_def)
-
-lemma get_view_closed:
-  assumes "reach tps_s s"
-    and "\<And>t. t \<in> wtxns_readable s cl (dom kv_map) \<Longrightarrow> closed' K (insert t (\<Union>k. get_view s cl k)) r"
-    and "cl_state (cls s cl) = RtxnInProg cclk (dom kv_map) kv_map"
-  shows "closed' K (\<Union>k \<in> dom kv_map. get_view s cl k) r"
-  using assms Rtxn_RegK_Kvtm_Cmt_in_rs_def[of s cl] Finite_Dom_Kv_map_rd_def[of s cl]
-  apply (auto intro!: Union_closed')
-  oops
-
-
-lemma cl_read_done_WR_onK:
-  assumes "reach tps_s s"
-    and "cl_read_done_s cl kv_map sn u'' clk s s'"
-  shows "R_onK WR (kvs_of_s s') = (wtxns_readable s cl (dom kv_map) \<times> {Tn (Tn_cl sn cl)}) \<union> R_onK WR (kvs_of_s s)"
-proof -
-  have reach_s': "reach tps_s s'"
-    using assms reach.reach_trans[of tps_s s "RDone cl kv_map sn u'' clk" s'] by auto
-  then show ?thesis
-    using assms cl_read_done_kvs_of_s[OF assms]
-    apply (auto simp add: R_onK_def WR_def full_view_def)
-    subgoal for k i t
-      using v_writer_kvs_of_s_nth[OF reach_s']
-      apply (auto simp add: tps_trans_defs wtxns_readable_def split: if_split_asm; intro exI[where x=k])
-        using v_writer_kvs_of_s_nth[OF assms(1)] Rtxn_Reads_Max_def[of s cl k]
-        apply (auto simp add: length_cts_order views_of_s_def)
-        by (metis image_eqI)+
-    subgoal by (metis image_eqI insertE)
-    subgoal apply (auto simp add: wtxns_readable_def)
-      subgoal for k 
-        apply (rule exI[where x=k], rule exI[where x="Max (views_of_s s cl k)"], auto)
-        using Max_views_of_s_in_range[OF assms(1)]
-          update_kv_v_writer_old[of "Max (views_of_s s cl k)" "kvs_of_s s" k]
-          v_writer_kvs_of_s_nth[OF assms(1)] Rtxn_Reads_Max_def[of s cl k]
-        by (auto simp add: full_view_def length_cts_order tps_trans_defs views_of_s_def).
-    subgoal for k i
-      apply (rule exI[where x=k], rule exI[where x=i])
-      by (auto simp add: full_view_def)
-    done
-qed
-
-lemma cl_read_done_extend_rel:
-  assumes "reach tps_s s"
-    and "cl_read_done_s cl kv_map sn u'' clk s s'"
-  shows "R_CC (kvs_of_s s') = (wtxns_readable s cl (dom kv_map) \<times> {Tn (Tn_cl sn cl)}) \<union> R_CC (kvs_of_s s)"
-  using assms
-  by (auto simp add: R_CC_def cl_read_done_WR_onK)
-           
-
-\<comment> \<open>cl_read_done closedness (canCommit)\<close>
-lemma cl_read_done_view_closed:
-  assumes "closed' (kvs_of_s s) (\<Union>k. get_view s cl' k) (R_CC (kvs_of_s s))"
-    and "kvs_writers (kvs_of_s s') = kvs_writers (kvs_of_s s)"
-    and "read_only_Txs (kvs_of_s s') = insert (Tn (get_txn s cl)) (read_only_Txs (kvs_of_s s))"
-    and "Tn (get_txn s cl) \<notin> ((R_CC (kvs_of_s s))\<inverse>)\<^sup>* ``
-      (visTx' (kvs_of_s s) (\<Union>k. get_view s cl' k))"
-    and "R_CC (kvs_of_s s') = (wtxns_readable s cl keys \<times> {Tn (get_txn s cl)}) \<union> R_CC (kvs_of_s s)"
-    and "Finite_Keys s cl"
-    and "cl_state (cls s cl) = RtxnInProg cclk keys kv_map"
-  shows "closed' (kvs_of_s s') (\<Union>k. get_view s cl' k) (R_CC (kvs_of_s s'))"
-  using assms visTx'_same_writers[OF assms(2)]
-  by (auto simp add: closed'_def visTx'_union_distr finite_wtxns_readable Finite_Keys_def
-    intro: closed_general_union_V_extend_N_extend_rel[where Y="wtxns_readable s cl keys"])
-                                                            
-\<comment> \<open>cl_write_commit closedness (canCommit)\<close>
-lemma cl_write_commit_WR_onK:
-  assumes "reach tps_s s"
-    and "cl_write_commit_s cl kv_map commit_t sn u'' clk mmap s s'"
-  shows "R_onK WR (kvs_of_s s') = R_onK WR (kvs_of_s s)"
-  using cl_write_commit_kvs_of_s[OF assms]
-  apply (auto simp add: R_onK_def WR_def full_view_def update_kv_defs split: if_split_asm)
-  apply blast
-  apply (metis (mono_tags, lifting) empty_iff full_view_append full_view_elemI image_eqI
-    less_SucE nth_append_length version.select_convs(3))
-  by (metis (no_types, lifting) full_view_elemI image_eqI less_Suc_eq update_kv_key_writes_simps)
-
-lemma cl_write_commit_same_rel:
-  assumes "reach tps_s s"
-    and "cl_write_commit_s cl kv_map cts sn u'' clk mmap s s'"
-  shows "R_CC (kvs_of_s s') = R_CC (kvs_of_s s)"
-  using assms
-  by (auto simp add: R_CC_def cl_write_commit_WR_onK)
-
-lemma "dom kv_map \<noteq> {} \<Longrightarrow> snd ` (\<Union>k\<in>dom kv_map. {(k, t)}) = {t}"
-  apply (auto simp add: image_def)
-  by (metis domIff insertI1 sndI)
-
-lemma cl_write_commit_view_closed:
-  assumes "reach tps_s s"
-    and "cl_write_commit_s cl kv_map cts sn u'' clk mmap s s'"
-    and "closed' (kvs_of_s s) (\<Union>k. get_view s cl k) (R_CC (kvs_of_s s))"
-    and "closed_general {get_wtxn s cl} ((R_CC (kvs_of_s s))\<inverse>)
-          (visTx' (kvs_of_s s) (\<Union>k. get_view s cl k) \<union> read_only_Txs (kvs_of_s s))"
-    and "read_only_Txs (kvs_of_s s') = read_only_Txs (kvs_of_s s)"
-    and "kvs_writers (kvs_of_s s') = insert (get_wtxn s cl) (kvs_writers (kvs_of_s s))"
-  shows "closed' (kvs_of_s s') (insert (get_wtxn s cl) (\<Union>k. get_view s cl k)) (R_CC (kvs_of_s s'))"
-  using assms
-  by (auto simp add: cl_write_commit_same_rel intro: insert_wr_t_closed')
-
 subsection \<open>Read-Only and Write-Only\<close>
 
 lemma fresh_t_notin_kvs_txids:
@@ -2380,12 +2103,313 @@ next
     case (RDone x1 x2 x3 x4 x5)
     then show ?case apply (auto simp add: SO_RO_WR_def tps_trans_defs SO_def SO0_def) sorry
   qed (auto simp add: SO_RO_WR_def tps_trans_defs)
+    qed
+    
+    
+subsection \<open>Closedness\<close>
+
+lemma visTx'_union_distr: "visTx' K (u\<^sub>1 \<union> u\<^sub>2) = visTx' K u\<^sub>1 \<union> visTx' K u\<^sub>2"
+  by (auto simp add: visTx'_def)
+
+lemma visTx'_Union_distr: "visTx' K (\<Union>i\<in>I. u i) = (\<Union>i\<in>I. visTx' K (u i))"
+  by (auto simp add: visTx'_def)
+
+lemma visTx'_same_writers: "kvs_writers K' = kvs_writers K \<Longrightarrow> visTx' K' u = visTx' K u"
+  by (simp add: visTx'_def)
+
+lemma union_closed':
+  assumes "closed' K u\<^sub>1 r"
+    and "closed' K u\<^sub>2 r"
+    and "kvs_writers K' = kvs_writers K" 
+    and "read_only_Txs K \<subseteq> read_only_Txs K'"
+  shows "closed' K' (u\<^sub>1 \<union> u\<^sub>2) r"
+  using assms
+  by (auto simp add: closed'_def visTx'_union_distr visTx'_same_writers[of K']
+           intro: closed_general_set_union_closed)
+
+lemma Union_closed':
+  assumes "\<And>i. i \<in> I \<Longrightarrow> closed' K (u i) r"
+    and "finite I" 
+    and "kvs_writers K' = kvs_writers K" 
+    and "read_only_Txs K \<subseteq> read_only_Txs K'"
+  shows "closed' K' (\<Union>i\<in>I. u i) r"
+  using assms                                  
+  apply (simp add: closed'_def visTx'_Union_distr visTx'_same_writers[of K'])
+  apply (rule closed_general_set_Union_closed)
+  apply auto
+  done
+
+lemma union_closed'_extend_rel:
+  assumes "closed' K u\<^sub>1 r"
+    and "closed' K u\<^sub>2 r"
+    and "kvs_writers K' = kvs_writers K" 
+    and "read_only_Txs K \<subseteq> read_only_Txs K'"
+    and "x \<notin> (r\<inverse>)\<^sup>* `` (visTx' K u\<^sub>1 \<union> visTx' K u\<^sub>2)"
+    and "r' = (\<Union>y\<in>Y. {(y, x)}) \<union> r"
+    and "finite Y"
+  shows "closed' K' (u\<^sub>1 \<union> u\<^sub>2) r'"
+  using assms
+  by (auto simp add: closed'_def visTx'_union_distr visTx'_same_writers[of K']
+      intro: closed_general_union_V_extend_N_extend_rel)
+
+
+lemma visTx'_new_writer: "kvs_writers K' = insert t (kvs_writers K) \<Longrightarrow>
+  visTx' K' (insert t u) = insert t (visTx' K u)"
+  by (auto simp add: visTx'_def)
+
+lemma insert_wr_t_closed':
+  assumes "closed' K u r"
+    and "closed_general {t} (r\<inverse>) (visTx' K u \<union> read_only_Txs K)"
+    and "read_only_Txs K' = read_only_Txs K"
+    and "kvs_writers K' = insert t (kvs_writers K)"
+  shows "closed' K' (insert t u) r"
+  using assms
+  by (auto simp add: closed'_def visTx'_new_writer intro: closed_general_set_union_closed)
+
+lemma visTx'_observes_t:
+  "t \<in> kvs_writers K \<Longrightarrow> visTx' K (insert t u) = insert t (visTx' K u)"
+  by (simp add: visTx'_def)
+
+lemma insert_kt_to_u_closed':
+  assumes "closed' K u r"
+    and "t \<in> kvs_writers K"
+    and "closed_general {t} (r\<inverse>) (visTx' K u \<union> read_only_Txs K)"
+  shows "closed' K (insert t u) r"
+  using assms
+  by (auto simp add: closed'_def visTx'_observes_t intro: closed_general_set_union_closed)
+ 
+lemma v_writer_kvs_of_s:
+  assumes "reach tps_s s"
+  shows "v_writer ` set (kvs_of_s s k) = set (cts_order s k)"
+  using assms CO_not_No_Ver_def[of s]
+  by (auto simp add: kvs_of_s_defs image_iff split: ver_state.split)
+
+lemma v_readerset_kvs_of_s:
+  assumes "reach tps_s s"
+  shows "\<Union> (v_readerset ` set (kvs_of_s s k)) = 
+   {t. \<exists>t_wr \<in> set (cts_order s k).
+      \<exists>cts sts lst v rs rts rlst. svr_state (svrs s k) t_wr = Commit cts sts lst v rs \<and>
+      rs t = Some (rts, rlst) \<and> get_sn t < cl_sn (cls s (get_cl t))}"
+  using assms CO_not_No_Ver_def[of s]
+  apply (auto simp add: kvs_of_s_defs split: ver_state.split ver_state.split_asm)
+  by blast
+
+lemma v_writer_kvs_of_s_nth:
+  "reach tps_s s \<Longrightarrow> i < length (kvs_of_s s k) \<Longrightarrow> v_writer (kvs_of_s s k ! i) = cts_order s k ! i"
+  using CO_not_No_Ver_def[of s k]
+  by (auto simp add: kvs_of_s_defs split: ver_state.split)
+
+lemma v_readerset_kvs_of_s_nth:
+  "reach tps_s s \<Longrightarrow> i < length (cts_order s k) \<Longrightarrow>
+    v_readerset (kvs_of_s s k ! i) = get_abst_rs s k (cts_order s k ! i)"
+  using CO_not_No_Ver_def[of s k]
+  by (auto simp add: kvs_of_s_defs split: ver_state.split)
+
+
+\<comment> \<open>cl_read_invoke_s\<close>
+definition RO_le_gst :: "'v global_conf \<Rightarrow> cl_id \<Rightarrow> txid set" where
+  "RO_le_gst s cl \<equiv> {t \<in> read_only_Txs (kvs_of_s s). \<exists>t'. t = Tn t' \<and> the (rtxn_rts s t') \<le> gst (cls s cl)}"
+
+lemma SO_trancl_SO_eq:
+  "SO\<^sup>+ = SO" 
+  apply (auto simp add: SO_def SO0_def)
+  subgoal
+    apply (induction rule: trancl_induct)
+    apply simp
+    by fastforce
+  done
+
+lemma get_view_incl_kvs_writers:
+  assumes "reach tps_s s"
+  shows "(\<Union>k. get_view s cl k) \<subseteq> kvs_writers (kvs_of_s s)"
+  using assms
+  apply (auto simp add: get_view_def)
+  using reach_co_not_no_ver set_cts_order_incl_kvs_writers by blast+
+
+
+abbreviation vis_RO where
+  "vis_RO s cl t \<equiv> (\<exists>x. t \<in> get_view s cl x) \<or> t \<in> RO_le_gst s cl"
+
+lemma cl_read_invoke_vis_RO_inv:
+  assumes "reach tps_s s"
+    and "reach tps_s s'"
+    and "(t, t') \<in> (R_CC (kvs_of_s s))\<^sup>+"
+    and "kvs_of_s s' = kvs_of_s s"
+  shows "vis_RO s' cl t' \<longrightarrow> vis_RO s' cl t"
+  using assms(3)
+  apply (induction t t' rule: trancl.induct)
+  subgoal for a b
+  apply (auto simp add: R_CC_def) sorry
+  subgoal for a b c 
+  apply (intro impI, elim impE, simp_all)
+  using assms(1,2,4)
+  apply (auto simp add: R_CC_def) sorry
+  done
+
+lemma get_view_closed:
+  assumes "reach tps_s s"
+    and "\<And>t. t \<in> wtxns_readable s cl (dom kv_map) \<Longrightarrow> closed' K (insert t (\<Union>k. get_view s cl k)) r"
+    and "cl_state (cls s cl) = RtxnInProg cclk (dom kv_map) kv_map"
+  shows "closed' K (\<Union>k \<in> dom kv_map. get_view s cl k) r"
+  using assms Rtxn_RegK_Kvtm_Cmt_in_rs_def[of s cl] Finite_Dom_Kv_map_rd_def[of s cl]
+  apply (auto intro!: Union_closed')
+  oops
+
+\<comment> \<open>cl_read_done_s\<close>
+lemma cl_read_done_same_writers:
+  assumes "reach tps_s s"
+    and "cl_read_done_s cl kv_map sn u'' clk s s'"
+  shows "kvs_writers (kvs_of_s s') = kvs_writers (kvs_of_s s)"
+proof -
+  have "reach tps_s s'"
+    using assms reach.reach_trans[of tps_s s "RDone cl kv_map sn u'' clk" s'] by auto
+  then show ?thesis
+    using assms CO_not_No_Ver_def[of s]
+    apply (simp add: kvs_writers_def vl_writers_def v_writer_kvs_of_s)
+    by (simp add: cl_read_done_s_def cl_read_done_U_def)
 qed
+
+lemma insert_Diff_if': "a \<notin> c \<Longrightarrow> insert a (b - c) = insert a b - c"
+  by (simp add: insert_Diff_if)
+
+lemma cl_read_done_t_notin_kvs_writers:
+  assumes "reach tps_s s"
+    and "cl_read_done_s cl kv_map sn u'' clk s s'"
+  shows "Tn (get_txn s cl) \<notin> kvs_writers (kvs_of_s s)"
+  using assms
+  apply (simp add: kvs_writers_def vl_writers_def v_writer_kvs_of_s)
+  using CO_Tid_def[of s cl] 
+  apply (auto simp add: tps_trans_defs)
+  by blast
+
+lemma UNIV_ex: "(\<Union>x. {t. P t x}) = ({t. \<exists>x. P t x})"
+  by auto
+
+lemma cl_read_done_new_read:
+  assumes "reach tps_s s"
+    and "cl_read_done_s cl kv_map sn u'' clk s s'"
+  shows "read_only_Txs (kvs_of_s s') = insert (Tn (get_txn s cl)) (read_only_Txs (kvs_of_s s))"
+proof -
+  have reach_s': "reach tps_s s'" 
+    using assms reach.reach_trans[of tps_s s "RDone cl kv_map sn u'' clk" s'] by auto
+  show ?thesis
+  using assms cl_read_done_t_notin_kvs_writers[OF assms] cl_read_done_same_writers[OF assms(1)]
+  apply (simp add: read_only_Txs_def insert_Diff_if')
+  apply (rule arg_cong[where f="\<lambda>m. m - _"])
+  apply (simp add: kvs_readers_def vl_readers_def v_readerset_kvs_of_s[OF assms(1)]
+      v_readerset_kvs_of_s[OF reach_s'] UNIV_ex)
+  using CO_not_No_Ver_def[of s']
+  apply (auto simp add: tps_trans_defs image_insert[symmetric] simp del: image_insert)
+  using image_eqI apply blast
+  apply (smt (z3) image_eqI insertCI less_SucE mem_Collect_eq txid0.collapse)
+  using image_eqI apply blast
+  subgoal apply (rule image_eqI, auto)
+    using Finite_Dom_Kv_map_rd_def[of s cl]
+    apply (cases "dom kv_map = {}", auto simp add: ex_in_conv[symmetric] simp del: dom_eq_empty_conv)
+    subgoal for k v apply (rule exI[where x=k])
+      using Rtxn_RegK_Kvtm_Cmt_in_rs_def[of s cl] Committed_Abs_in_CO_def[of s]
+      apply (auto simp add: is_committed_in_kvs_def)
+      by (metis (no_types, lifting) is_committed.simps(1))
+    done
+  by (smt (verit) image_eqI less_Suc_eq mem_Collect_eq)
+qed
+
+definition wtxns_readable :: "('v, 'm) global_conf_scheme \<Rightarrow> cl_id \<Rightarrow> key set \<Rightarrow> txid set" where
+  "wtxns_readable s cl keys \<equiv> {read_at (svr_state (svrs s k)) (gst (cls s cl)) cl | k. k \<in> keys}"
+
+lemma finite_wtxns_readable: "finite keys \<longrightarrow> finite (wtxns_readable s cl keys)"
+  by (simp add: wtxns_readable_def)
+
+lemma cl_read_done_WR_onK:
+  assumes "reach tps_s s"
+    and "cl_read_done_s cl kv_map sn u'' clk s s'"
+  shows "R_onK WR (kvs_of_s s') = (wtxns_readable s cl (dom kv_map) \<times> {Tn (Tn_cl sn cl)}) \<union> R_onK WR (kvs_of_s s)"
+proof -
+  have reach_s': "reach tps_s s'"
+    using assms reach.reach_trans[of tps_s s "RDone cl kv_map sn u'' clk" s'] by auto
+  then show ?thesis
+    using assms cl_read_done_kvs_of_s[OF assms]
+    apply (auto simp add: R_onK_def WR_def full_view_def)
+    subgoal for k i t
+      using v_writer_kvs_of_s_nth[OF reach_s']
+      apply (auto simp add: tps_trans_defs wtxns_readable_def split: if_split_asm; intro exI[where x=k])
+        using v_writer_kvs_of_s_nth[OF assms(1)] Rtxn_Reads_Max_def[of s cl k]
+        apply (auto simp add: length_cts_order views_of_s_def)
+        by (metis image_eqI)+
+    subgoal by (metis image_eqI insertE)
+    subgoal apply (auto simp add: wtxns_readable_def)
+      subgoal for k 
+        apply (rule exI[where x=k], rule exI[where x="Max (views_of_s s cl k)"], auto)
+        using Max_views_of_s_in_range[OF assms(1)]
+          update_kv_v_writer_old[of "Max (views_of_s s cl k)" "kvs_of_s s" k]
+          v_writer_kvs_of_s_nth[OF assms(1)] Rtxn_Reads_Max_def[of s cl k]
+        by (auto simp add: full_view_def length_cts_order tps_trans_defs views_of_s_def).
+    subgoal for k i
+      apply (rule exI[where x=k], rule exI[where x=i])
+      by (auto simp add: full_view_def)
+    done
+qed
+
+lemma cl_read_done_extend_rel:
+  assumes "reach tps_s s"
+    and "cl_read_done_s cl kv_map sn u'' clk s s'"
+  shows "R_CC (kvs_of_s s') = (wtxns_readable s cl (dom kv_map) \<times> {Tn (Tn_cl sn cl)}) \<union> R_CC (kvs_of_s s)"
+  using assms
+  by (auto simp add: R_CC_def cl_read_done_WR_onK)
+
+
+lemma cl_read_done_view_closed:
+  assumes "closed' (kvs_of_s s) (\<Union>k. get_view s cl' k) (R_CC (kvs_of_s s))"
+    and "kvs_writers (kvs_of_s s') = kvs_writers (kvs_of_s s)"
+    and "read_only_Txs (kvs_of_s s') = insert (Tn (get_txn s cl)) (read_only_Txs (kvs_of_s s))"
+    and "Tn (get_txn s cl) \<notin> ((R_CC (kvs_of_s s))\<inverse>)\<^sup>* ``
+      (visTx' (kvs_of_s s) (\<Union>k. get_view s cl' k))"
+    and "R_CC (kvs_of_s s') = (wtxns_readable s cl keys \<times> {Tn (get_txn s cl)}) \<union> R_CC (kvs_of_s s)"
+    and "Finite_Keys s cl"
+    and "cl_state (cls s cl) = RtxnInProg cclk keys kv_map"
+  shows "closed' (kvs_of_s s') (\<Union>k. get_view s cl' k) (R_CC (kvs_of_s s'))"
+  using assms visTx'_same_writers[OF assms(2)]
+  by (auto simp add: closed'_def visTx'_union_distr finite_wtxns_readable Finite_Keys_def
+    intro: closed_general_union_V_extend_N_extend_rel[where Y="wtxns_readable s cl keys"])
+                                                            
+\<comment> \<open>cl_write_commit_s\<close>
+lemma cl_write_commit_WR_onK:
+  assumes "reach tps_s s"
+    and "cl_write_commit_s cl kv_map commit_t sn u'' clk mmap s s'"
+  shows "R_onK WR (kvs_of_s s') = R_onK WR (kvs_of_s s)"
+  using cl_write_commit_kvs_of_s[OF assms]
+  apply (auto simp add: R_onK_def WR_def full_view_def update_kv_defs split: if_split_asm)
+  apply blast
+  apply (metis (mono_tags, lifting) empty_iff full_view_append full_view_elemI image_eqI
+    less_SucE nth_append_length version.select_convs(3))
+  by (metis (no_types, lifting) full_view_elemI image_eqI less_Suc_eq update_kv_key_writes_simps)
+
+lemma cl_write_commit_same_rel:
+  assumes "reach tps_s s"
+    and "cl_write_commit_s cl kv_map cts sn u'' clk mmap s s'"
+  shows "R_CC (kvs_of_s s') = R_CC (kvs_of_s s)"
+  using assms
+  by (auto simp add: R_CC_def cl_write_commit_WR_onK)
+
+lemma "dom kv_map \<noteq> {} \<Longrightarrow> snd ` (\<Union>k\<in>dom kv_map. {(k, t)}) = {t}"
+  apply (auto simp add: image_def)
+  by (metis domIff insertI1 sndI)
+
+
+lemma cl_write_commit_view_closed:
+  assumes "reach tps_s s"
+    and "cl_write_commit_s cl kv_map cts sn u'' clk mmap s s'"
+    and "closed' (kvs_of_s s) (\<Union>k. get_view s cl' k) (R_CC (kvs_of_s s))"
+    and "closed_general {get_wtxn s cl} ((R_CC (kvs_of_s s))\<inverse>)
+          (visTx' (kvs_of_s s) (\<Union>k. get_view s cl' k) \<union> read_only_Txs (kvs_of_s s))"
+    and "read_only_Txs (kvs_of_s s') = read_only_Txs (kvs_of_s s)"
+    and "kvs_writers (kvs_of_s s') = insert (get_wtxn s cl) (kvs_writers (kvs_of_s s))"
+  shows "closed' (kvs_of_s s') (insert (get_wtxn s cl) (\<Union>k. get_view s cl' k)) (R_CC (kvs_of_s s'))"
+  using assms
+  by (auto simp add: cl_write_commit_same_rel intro: insert_wr_t_closed')
 
 
 subsection \<open>CanCommit\<close>
-
-lemmas canCommit_defs = ET_CC.canCommit_def R_CC_def R_onK_def
 
 lemma visTx_visTx':
   assumes "reach tps_s s"
@@ -2411,16 +2435,9 @@ lemma closed_closed':
     closed' (kvs_of_s s) (\<Union>k. get_view s cl k) r"
   by (simp add: closed'_def visTx_visTx')
 
-lemma visTx'_cl_ctx_subset_writers:
-  "visTx' (kvs_of_s s) (cl_ctx (cls s cl)) \<subseteq> kvs_writers (kvs_of_s s)"
-  by (simp add: visTx'_def)
-
 lemma visTx'_subset_writers: 
   "visTx' (kvs_of_s s) u \<subseteq> kvs_writers (kvs_of_s s)"
   by (simp add: visTx'_def)
-
-definition RO_le_gst :: "'v global_conf \<Rightarrow> cl_id \<Rightarrow> txid set" where
-  "RO_le_gst s cl \<equiv> {t \<in> read_only_Txs (kvs_of_s s). \<exists>t'. t = Tn t' \<and> the (rtxn_rts s t') \<le> gst (cls s cl)}"
 
 definition PTid_In_KVS where
   "PTid_In_KVS s cl \<longleftrightarrow> (case cl_state (cls s cl) of
@@ -2483,6 +2500,23 @@ proof -
     by (auto split: txn_state.split_asm)
 qed
 
+lemma bla:
+  assumes "reach tps_s s"
+    and "(a, b) \<in> SO"
+    and "b \<in> (\<Union>k. get_view s cl k)"
+    and "a \<notin> read_only_Txs (kvs_of_s s)"
+  shows "a \<in> (\<Union>k. get_view s cl k)"
+proof -
+  have "a \<in> kvs_writers (kvs_of_s s)"
+    using assms get_view_incl_kvs_writers[OF assms(1)]
+      kvs_writers_readers_disjoint[OF assms(1)]
+      SO_in_kvs_txids[OF assms(1)]
+    apply (auto simp add: SO_def SO0_def kvs_txids_def read_only_Txs_def)
+    by (metis assms(3) subset_iff)
+  then show ?thesis using assms
+    apply (auto simp add: get_view_def')
+    oops
+
 
 subsection \<open>Views\<close>
 
@@ -2503,7 +2537,7 @@ lemmas get_view_update_lemmas =
   get_view_update_cls get_view_update_cls_rtxn_rts
 
 
-subsubsection \<open>View Invariants\<close>
+subsubsection \<open>View Closed\<close>
 
 lemma get_view_init: "get_view state_init cl = (\<lambda>k. {T0})"
   by (auto simp add: tps_s_defs get_view_def)
@@ -2512,59 +2546,6 @@ lemma Union_image_map:
   "\<Union> (f ` {x. m x = None}) \<union> \<Union> (f ` {x. \<exists>y. m x = Some y}) = (\<Union>x. f x)"
   apply auto
   by blast
-
-lemma get_view_incl_kvs_writers:
-  assumes "reach tps_s s"
-  shows "(\<Union>k. get_view s cl k) \<subseteq> kvs_writers (kvs_of_s s)"
-  using assms
-  apply (auto simp add: get_view_def)
-  using reach_co_not_no_ver set_cts_order_incl_kvs_writers by blast+
-
-lemma SO_trancl_SO_eq:
-  "SO\<^sup>+ = SO" 
-  apply (auto simp add: SO_def SO0_def)
-  subgoal
-    apply (induction rule: trancl_induct)
-    apply simp
-    by fastforce
-  done
-
-lemma bla:
-  assumes "reach tps_s s"
-    and "(a, b) \<in> SO"
-    and "b \<in> (\<Union>k. get_view s cl k)"
-    and "a \<notin> read_only_Txs (kvs_of_s s)"
-  shows "a \<in> (\<Union>k. get_view s cl k)"
-proof -
-  have "a \<in> kvs_writers (kvs_of_s s)"
-    using assms get_view_incl_kvs_writers[OF assms(1)]
-      kvs_writers_readers_disjoint[OF assms(1)]
-      SO_in_kvs_txids[OF assms(1)]
-    apply (auto simp add: SO_def SO0_def kvs_txids_def read_only_Txs_def)
-    by (metis assms(3) subset_iff)
-  then show ?thesis using assms
-    apply (auto simp add: get_view_def')
-    sorry
-qed
-
-abbreviation vis_RO where
-  "vis_RO s cl t \<equiv> (\<exists>x. t \<in> get_view s cl x) \<or> t \<in> RO_le_gst s cl"
-
-lemma cl_read_invoke_vis_RO_inv:
-  assumes "reach tps_s s"
-    and "reach tps_s s'"
-    and "(t, t') \<in> (R_CC (kvs_of_s s))\<^sup>+"
-    and "kvs_of_s s' = kvs_of_s s"
-  shows "vis_RO s' cl t' \<longrightarrow> vis_RO s' cl t"
-  using assms(3)
-  apply (induction t t' rule: trancl.induct)
-  subgoal for a b
-  apply (auto simp add: R_CC_def) sorry
-  subgoal for a b c 
-  apply (intro impI, elim impE, simp_all)
-  using assms(1,2,4)
-  apply (auto simp add: R_CC_def) sorry
-  done
 
 lemma vis_Tx'_get_view:
   "reach tps_s s \<Longrightarrow> visTx' (kvs_of_s s) (\<Union>k. get_view s cl k) = (\<Union>k. get_view s cl k)"
@@ -2627,28 +2608,35 @@ next
       by (auto simp add: next_txids_def get_sqns_old_def kvs_txids_def visTx'_def)
   next
     case (WCommit x1 x2 x3 x4 x5 x6 x7)
+    then have a:  "cl_sn (cls s x1) = x4" "Tn_cl x4 x1 \<in> next_txids (kvs_of_s s) x1"
+      using t_is_fresh[OF WCommit(2)] by (auto simp add: tps_trans_defs)
     then show ?case
     proof (cases "x1 = cl")
       case True
-      then have "Tn_cl x4 x1 \<in> next_txids (kvs_of_s s) x1"
-        using t_is_fresh[OF WCommit(2)] WCommit(1) by (auto simp add: tps_trans_defs)
-      then show ?thesis using WCommit True
+      then show ?thesis using WCommit a
           cl_write_commit_get_view[OF WCommit(2,1)[simplified]]
         apply (auto simp add: View_Closed_def)
-        subgoal sorry
-        subgoal apply (simp add: Union_image_map[of "get_view s cl" x2])
+        subgoal
+          using cl_write_commit_same_rel[OF WCommit(2,1)[simplified]]
+            cl_write_commit_kvs_of_s[OF WCommit(2,1)[simplified]]
+          by (auto simp add: closed'_def visTx'_def kvs_writers_update_kv read_only_Txs_update_kv)
+        subgoal
+          apply (simp add: Union_image_map[of "get_view s cl" x2])
+          apply (intro cl_write_commit_view_closed, simp_all)
           using cl_write_commit_kvs_of_s[OF WCommit(2,1)[simplified]]
-          apply (intro cl_write_commit_view_closed)
           apply (auto simp add: kvs_writers_update_kv read_only_Txs_update_kv)
-          subgoal
-            apply (auto simp add: closed'_def closed_general_def visTx'_def 
-                kvs_writers_def vl_writers_def v_writer_kvs_of_s trancl_converse) sorry
-          by (simp_all add: tps_trans_defs)
+          apply (auto simp add: closed_general_def) sorry
         done
     next
       case False
-      then show ?thesis using WCommit
-      apply (auto simp add: View_Closed_def) sorry
+      then show ?thesis using WCommit a(2)
+          cl_write_commit_get_view[OF WCommit(2,1)[simplified]]
+          cl_write_commit_same_rel[OF WCommit(2,1)[simplified]]
+          cl_write_commit_kvs_of_s[OF WCommit(2,1)[simplified]]
+        apply (auto simp add: View_Closed_def closed'_def visTx'_def
+            kvs_writers_update_kv read_only_Txs_update_kv)
+        by (metis (no_types, lifting) Int_iff Int_insert_left_if0
+            insert_absorb visTx'_def vis_Tx'_get_view)
     qed
   qed (simp_all add: View_Closed_def tps_trans_defs)
 qed
